EthCryptographySpecs/Proofs/Kzg.lean
@@ -1,6 +1,7 @@
 import EthCryptographySpecs.Proofs.Kzg.BitReversal
 import EthCryptographySpecs.Proofs.Kzg.Fft
 import EthCryptographySpecs.Proofs.Kzg.Polynomials
+import EthCryptographySpecs.Proofs.Kzg.Core
 
 /-!
 # `EthCryptographySpecs.Proofs.Kzg`
